Add iota-reduction tests, regen logs

coq/PerformanceExperiments/aggregate.py
@@ -19,7 +19,10 @@ def process_file(f, data):
     def param_to_tuple(p):
         k, v = p.split('=')
         if k.startswith(REPLACE_KEY): return (k, v.split('|'))
-        return (k, int(v))
+        try:
+            return (k, int(v))
+        except ValueError:
+            return (k, v)
     reg = re.compile(r'(?:Tactic call|Finished) (.*?) (?:ran for|in) ([0-9\.]+) secs \(([0-9\.]+)u,([0-9\.]+)s\)(?: \(success\)| \(successful\))?')
     fdir, fname = os.path.split(f.name)
     fbase, kind = os.path.split(fdir)
