coq/PerformanceExperiments/iota_reduction_common.v
@@ -1,0 +1,46 @@
+Require Import PerformanceExperiments.Harness.
+
+Fixpoint fact (n : nat) := match n with 0 => 1 | S n' => n * fact n' end.
+Fixpoint walk (n : nat) : unit := match n with 0 => tt | S n => walk n end.
+Definition skip (n : nat) : unit := tt.
+Inductive value := the (A : Type) (_ : A).
+Arguments the : clear implicits.
+Notation slown n := (the (walk (fact n) = tt) (eq_refl tt)) (only parsing).
+Notation fastn n := (the (skip (fact n) = tt) (eq_refl tt)) (only parsing).
+
+Notation iota_the v := match v return value with
+                       | the A a => the A a
+                       end.
+
+Inductive speed := slow | fast.
+Ltac describe_goal_gen factn speed n := idtac "Params: a-n=" n ", fact-n=" factn (* ", speed=" speed*).
+Ltac step_goal_constr _ v := uconstr:(iota_the v).
+Ltac redgoal_constr _ v := constr:(v).
+Ltac time_solve_goal_gen_slow with_abstract n v :=
+  optimize_heap;
+  restart_timer;
+  let v2 := (eval cbv beta iota in v) in
+  finish_timing ("Tactic call beta-iota-slow");
+  time "unify-beta-iota-slow" unify v v2;
+  lazymatch with_abstract with
+  | true => let __ := constr:(ltac:(time "abstract-unify-beta-iota-slow" abstract exact_no_check (eq_refl v)) : v = v2) in
+            idtac
+  | false => idtac
+  end.
+Ltac time_solve_goal_gen_fast with_abstract n v :=
+  optimize_heap;
+  restart_timer;
+  let v2 := (eval cbv beta iota in v) in
+  finish_timing ("Tactic call beta-iota-fast");
+  time "unify-beta-iota-fast" unify v v2;
+  lazymatch with_abstract with
+  | true => let __ := constr:(ltac:(time "abstract-unify-beta-iota-fast" abstract exact_no_check (eq_refl v)) : v = v2) in
+            idtac
+  | false => idtac
+  end.
+Ltac mkgoal_init speed factn :=
+  let factn := (eval cbv in (Z.to_nat factn)) in
+  lazymatch speed with
+  | slow => constr:(slown factn)
+  | fast => constr:(fastn factn)
+  end.
