coq/PerformanceExperiments/iota_reduction_with_abstract_fact8.v
@@ -1,0 +1,29 @@
+Require Import PerformanceExperiments.Harness.
+Require Export PerformanceExperiments.iota_reduction_common.
+
+Global Open Scope Z_scope.
+
+Local Notation factn := 8.
+Local Notation with_abstract := true.
+
+Definition args_of_size (s : size) : list Z
+  := match s with
+     | Sanity => List.map Z.of_nat (seq 0 3)
+     | SuperFast => List.map (fun x => Z.of_nat x * 100) (seq 1 10)
+     | Fast => List.map (fun x => Z.of_nat x * 100) (seq 1 100)
+     | Medium => []
+     | Slow => []
+     | VerySlow => []
+     end.
+
+Ltac describe_goal0 n := describe_goal_gen constr:(factn) slow n.
+Ltac time_solve_goal0 n v := time_solve_goal_gen_slow constr:(with_abstract) n v.
+Ltac run0 sz := idtac; Harness.runtests_step_constr args_of_size describe_goal0 step_goal_constr redgoal_constr time_solve_goal0 sz ltac:(mkgoal_init slow constr:(factn)).
+
+Ltac describe_goal1 n := describe_goal_gen constr:(factn) fast n.
+Ltac time_solve_goal1 n v := time_solve_goal_gen_fast constr:(with_abstract) n v.
+Ltac run1 sz := Harness.runtests_step_constr args_of_size describe_goal1 step_goal_constr redgoal_constr time_solve_goal1 sz ltac:(mkgoal_init fast constr:(factn)).
+
+(*
+Goal True. run0 Fast.
+*)
